Tests/All.lean
@@ -1,6 +1,9 @@
 import Tests.Lexer
 import Tests.Golden
+import Tests.IR
+import Tests.PublicInterface
 
 def main : IO Unit := do
   lexerMain
+  irMain
   goldenMain
